# The Fibonacci sequence

```agda
module elementary-number-theory.fibonacci-sequence where
```

<details><summary>Imports</summary>

```agda
open import elementary-number-theory.addition-natural-numbers
open import elementary-number-theory.natural-numbers
```

</details>

```agda
Fibonacci-ℕ : ℕ → ℕ
Fibonacci-ℕ 0 = 0
Fibonacci-ℕ (succ-ℕ 0) = 1
Fibonacci-ℕ (succ-ℕ (succ-ℕ n)) = add-ℕ (Fibonacci-ℕ (succ-ℕ n)) (Fibonacci-ℕ n)
```

The above definition of the Fibonacci sequence uses Agda's powerful
pattern matching definitions. Below, we will give a definition of the
Fibonacci sequence in terms of `ind-ℕ`.

The problem with defining the Fibonacci sequence using `ind-ℕ`, is that `ind-ℕ`
doesn't give us a way to refer to both `(F n)` and `(F (succ-ℕ n))`. So, we have
to give a workaround, where we store two values in the Fibonacci sequence
at once.

The basic idea is that we define a sequence of pairs of integers, which will
be consecutive Fibonacci numbers. This would be a function of type $ℕ → ℕ²$.

Such a function is easy to give with induction, using the map $ℕ² → ℕ²$ that
takes a pair `(m,n)` to the pair `(n,n+m)`. Starting the iteration with `(0,1)`
we obtain the Fibonacci sequence by taking the first projection.

However, we haven't defined cartesian products or booleans yet. Therefore
we mimic the above idea, using $ℕ → ℕ$ instead of $ℕ²$.

```agda
shift-one : ℕ → (ℕ → ℕ) → (ℕ → ℕ)
shift-one n f = ind-ℕ n (λ x y → f x)

shift-two : ℕ → ℕ → (ℕ → ℕ) → (ℕ → ℕ)
shift-two m n f = shift-one m (shift-one n f)

Fibo-zero-ℕ : ℕ → ℕ
Fibo-zero-ℕ = shift-two 0 1 (λ x → 0)

Fibo-succ-ℕ : (ℕ → ℕ) → (ℕ → ℕ)
Fibo-succ-ℕ f = shift-two (f 1) (add-ℕ (f 1) (f 0)) (λ x → 0)

Fibo-function : ℕ → ℕ → ℕ
Fibo-function =
  ind-ℕ
    ( Fibo-zero-ℕ)
    ( λ n → Fibo-succ-ℕ)

Fibo : ℕ → ℕ
Fibo k = Fibo-function k 0
```
